Weidenbach_Book/IsaSAT/IsaSAT_Setup0_LLVM.thy
@@ -47,7 +47,7 @@ type_synonym twl_st_wll_trail_fast2 =
 
 definition isasat_bounded_assn :: \<open>isasat \<Rightarrow> twl_st_wll_trail_fast2 \<Rightarrow> assn\<close> where
 \<open>isasat_bounded_assn = tuple17_assn
-  trail_pol_fast_assn  arena_fast_assn
+  trail_pol_fast_assn arena_fast_assn
   conflict_option_rel_assn
   sint64_nat_assn
   watchlist_fast_assn
@@ -173,7 +173,7 @@ lemma [sepref_fr_rules]: \<open>(uncurry0 (Mreturn 0), uncurry0 (RETURN bottom_a
   by (smt (verit, best) pure_true_conv rel_simps(51) sep.add_0)
 
 definition bottom_bump :: \<open>bump_heuristics\<close> where
-  \<open>bottom_bump = Tuple4 bottom_vmtf bottom_vmtf False bottom_atms_hash\<close>
+  \<open>bottom_bump = Tuple4 empty_acids bottom_vmtf False bottom_atms_hash\<close>
 
 definition extract_vmtf_wl_heur where
   \<open>extract_vmtf_wl_heur = isasat_state_ops.remove_f bottom_bump\<close>
